Prove correctness of loop generation

Instr.v
@@ -1,5 +1,26 @@
 Require Import ZArith.
+Require Import Psatz.
+
+Open Scope Z_scope.
 
 Parameter instr : Type.
 Parameter mem : Type.
 Parameter instr_semantics : instr -> list Z -> mem -> mem -> Prop.
+
+Inductive iter_semantics (P : Z -> mem -> mem -> Prop) : Z -> Z -> mem -> mem -> Prop :=
+| IDone : forall lb ub mem, ub <= lb -> iter_semantics P lb ub mem mem
+| IProgress : forall lb ub mem1 mem2 mem3,
+    lb < ub -> P lb mem1 mem2 -> iter_semantics P (lb + 1) ub mem2 mem3 ->
+    iter_semantics P lb ub mem1 mem3.
+
+Lemma iter_semantics_map (P Q : Z -> mem -> mem -> Prop) :
+  forall lb ub mem1 mem2,
+    (forall x mem1 mem2, lb <= x < ub -> P x mem1 mem2 -> Q x mem1 mem2) ->
+    iter_semantics P lb ub mem1 mem2 ->
+    iter_semantics Q lb ub mem1 mem2.
+Proof.
+  intros lb ub mem1 mem2 Himp Hsem.
+  induction Hsem; econstructor; eauto; [eapply Himp|eapply IHHsem]; eauto.
+  - lia.
+  - intros; apply Himp; auto; lia.
+Qed.
