CodeGen.v
@@ -4,10 +4,13 @@ Require Import ZArith.
 Require Import List.
 Require Import Bool.
 Require Import Psatz.
+Require Import Setoid Morphisms.
 
 Require Import Linalg.
 Require Import Loop.
 Require Import PolyLang.
+Require Import Misc.
+Require Import Instr.
 
 Open Scope Z_scope.
 Open Scope list_scope.
@@ -95,11 +98,68 @@ Fixpoint make_linear_expr (n : nat) (l : list Z) :=
   | S n, x :: l => Sum (Mult x (Var n)) (make_linear_expr n l)
   end.
 
+Lemma firstn_nth_app :
+  forall A n (l : list A) d, (length l >= S n)%nat -> firstn (S n) l = firstn n l ++ (nth n l d :: nil).
+Proof.
+  intros A. induction n.
+  - intros l d H; destruct l; simpl in *; [lia | auto].
+  - intros l d H; destruct l; simpl in *; [lia |].
+    erewrite IHn by lia. reflexivity.
+Qed.
+
+Theorem make_linear_expr_correct_aux :
+  forall n l env, (length env >= n)%nat -> eval_expr env (make_linear_expr n l) = dot_product l (rev (firstn n env)).
+Proof.
+  induction n.
+  - intros l env Hel. destruct env; destruct l; simpl in *; auto; lia.
+  - intros l env Hel.
+    destruct l as [|x l]; simpl in Hel; destruct (rev (firstn (S n) env)) as [|y ev] eqn:Hrev; auto; simpl; auto.
+    + destruct env as [|e env]; simpl in *; [lia | destruct (rev (firstn n env)); simpl in *; congruence].
+    + rewrite firstn_nth_app with (d := 0) in Hrev by auto. rewrite rev_unit in Hrev.
+      injection Hrev as Hnth Hrev. rewrite IHn by lia. congruence.
+Qed.
+
+Theorem make_linear_expr_correct :
+  forall n l env, length env = n -> eval_expr env (make_linear_expr n l) = dot_product l (rev env).
+Proof.
+  intros. rewrite make_linear_expr_correct_aux by lia. f_equal. f_equal. apply firstn_all2. lia.
+Qed.
+
 Definition make_affine_expr (n : nat) (e : (vector * Z)%type) := Sum (make_linear_expr n (fst e)) (Constant (snd e)).
+
+Theorem make_affine_expr_correct :
+  forall n e env, length env = n -> eval_expr env (make_affine_expr n e) = dot_product (fst e) (rev env) + snd e.
+Proof.
+  intros. simpl in *. rewrite make_linear_expr_correct; auto.
+Qed.
 
 Parameter project : nat -> polyhedron -> result polyhedron.
 Parameter find_lower_bound : nat -> polyhedron -> result expr.
 Parameter find_upper_bound : nat -> polyhedron -> result expr.
+
+Axiom project_inclusion :
+  forall n p pol proj, project n pol = Ok proj -> in_poly p pol = true -> in_poly (resize n p) proj = true.
+Axiom project_reverse_inclusion :
+  forall n pol proj c, project n pol = Ok proj -> In c pol -> fst c =v= resize n (fst c) -> (exists c', c =c= c' /\ In c' proj).
+
+Axiom find_lower_bound_correct :
+  forall n pol env x lb, find_lower_bound n pol = Ok lb -> length env = n ->
+                    eval_expr env lb <= x <-> (forall c, In c pol -> nth n (fst c) 0 < 0 -> satisfies_constraint (rev env ++ x :: nil) c = true).
+Axiom find_upper_bound_correct :
+  forall n pol env x ub, find_upper_bound n pol = Ok ub -> length env = n ->
+                    x < eval_expr env ub <-> (forall c, In c pol -> nth n (fst c) 0 > 0 -> satisfies_constraint (rev env ++ x :: nil) c = true).
+
+Theorem find_bounds_correct :
+  forall n pol env x lb ub, find_lower_bound n pol = Ok lb -> find_upper_bound n pol = Ok ub -> length env = n ->
+                       eval_expr env lb <= x < eval_expr env ub <-> (forall c, In c pol -> nth n (fst c) 0 <> 0 -> satisfies_constraint (rev env ++ x :: nil) c = true).
+Proof.
+  intros n pol env x lb ub Hlb Hub Hlen.
+  rewrite find_lower_bound_correct; eauto.
+  rewrite find_upper_bound_correct; eauto.
+  split.
+  - intros [H1 H2] c Hin Hnotzero. destruct (nth n (fst c) 0 <=? 0) eqn:Hcmp; reflect; [apply H1 | apply H2]; auto; lia.
+  - intros H; split; intros c Hin Hcmp; apply H; auto; lia.
+Qed.
 
 Fixpoint generate_loop (d : nat) (n : nat) (pi : Polyhedral_Instruction) : result stmt :=
   match d with
@@ -112,32 +172,169 @@ Fixpoint generate_loop (d : nat) (n : nat) (pi : Polyhedral_Instruction) : resul
     Ok (Loop lb ub inner)
   end.
 
-Theorem generate_loop_preserves_sem :
-  forall st env mem1 mem2,
-    loop_semantics st env mem1 mem2 ->
-    forall pi d n,
-      generate_loop d n pi = Ok st ->
-      length env = (n - d)%nat ->
-      (forall c, In c pi.(pi_poly) -> (length (fst c) <= n)%nat) ->
-      env_poly_lex_semantics (rev env) n (pi :: nil) mem1 mem2.
+Lemma env_scan_begin :
+  forall polys env n p m, env_scan polys env n m p = true -> p =v= env ++ skipn (length env) p.
 Proof.
-  intros st env mem1 mem2 Hsem. induction Hsem.
-  - intros pi d n Hgen Hlen Hpilen.
-    destruct d; simpl in *; inversion Hgen.
-    + unfold env_poly_lex_semantics.
-      eapply PolyLexProgress with (n := 0%nat) (p := rev env); [ |reflexivity| | | apply PolyLexDone].
-      * admit.
-      * admit.
-    + bind_ok_destruct Hgen proj Hproj.
-      bind_ok_destruct Hgen lb Hlb.
-      bind_ok_destruct Hgen ub Hub.
-      bind_ok_destruct Hgen inner Hinner.
-      inversion Hgen.
-  - intros pi d n Hgen Hlen; destruct d; simpl in *; [inversion Hgen|].
-    bind_ok_destruct Hgen proj Hproj.
-    bind_ok_destruct Hgen lb Hlb.
-    bind_ok_destruct Hgen ub Hub.
-    bind_ok_destruct Hgen inner Hinner.
-    inversion Hgen.
-  - admit.
-Admitted.
+  intros polys env n p m Hscan. unfold env_scan in Hscan. destruct (nth_error polys m); [|congruence].
+  reflect. destruct Hscan as [[Heq1 Heq2] Heq3].
+  apply same_length_eq in Heq1; [|rewrite resize_length; auto].
+  rewrite Heq1 at 1.
+  rewrite resize_skipn_eq; reflexivity.
+Qed.
+  
+Lemma env_scan_single :
+  forall polys env n p m, length env = n -> env_scan polys env n m p = true -> env =v= p.
+Proof.
+  intros polys env n p m Hlen Hscan.
+  unfold env_scan in Hscan. destruct (nth_error polys m); [|congruence].
+  reflect. destruct Hscan as [[Heq1 Heq2] Heq3]. rewrite Hlen in Heq1.
+  rewrite Heq1. symmetry. auto.
+Qed.
+
+Lemma nth_skipn :
+  forall A n m (l : list A) d, nth n (skipn m l) d = nth (m + n) l d.
+Proof.
+  induction m.
+  - intros. simpl. reflexivity.
+  - intros. simpl.
+    destruct l; simpl.
+    + destruct n; reflexivity.
+    + apply IHm.
+Qed.
+
+Lemma env_scan_split :
+  forall polys env n p m, (length env < n)%nat -> env_scan polys env n m p = true <-> (exists x, env_scan polys (env ++ (x :: nil)) n m p = true).
+Proof.
+  intros polys env n p m Hlen.
+  unfold env_scan. destruct (nth_error polys m); simpl; [|split; [intros; congruence|intros [x Hx]; auto]].
+  split.
+  - intros H. exists (nth (length env) p 0).
+    reflect. destruct H as [[H1 H2] H3].
+    split; [split|]; auto.
+    rewrite app_length. simpl. rewrite <- resize_skipn_eq with (l := p) (d := length env) at 2.
+    rewrite resize_app_le by (rewrite resize_length; lia).
+    rewrite resize_length. rewrite <- is_eq_veq.
+    rewrite is_eq_app by (rewrite resize_length; auto).
+    reflect; split; auto.
+    replace (length env + 1 - length env)%nat with 1%nat by lia.
+    simpl. transitivity (nth 0 (skipn (length env) p) 0 :: nil).
+    + rewrite nth_skipn. rewrite Nat.add_0_r. reflexivity.
+    + destruct (skipn (length env) p); simpl; reflexivity.
+  - intros [x Hx]. reflect. destruct Hx as [[H1 H2] H3].
+    + split; [split|]; auto.
+      rewrite app_length in H1. simpl in H1.
+      rewrite <- is_eq_veq in H1. rewrite is_eq_app_left in H1.
+      reflect; destruct H1 as [H1 H4]. rewrite resize_resize in H1 by lia. assumption.
+Qed.
+
+Lemma resize_succ :
+  forall n l, resize (S n) l = resize n l ++ nth n l 0 :: nil.
+Proof.
+  induction n.
+  - intros; destruct l; simpl; auto.
+  - intros; destruct l; simpl in *; f_equal.
+    + rewrite (IHn nil). destruct n; auto.
+    + apply IHn.
+Qed.
+
+Theorem nth_eq :
+  forall n l1 l2, l1 =v= l2 -> nth n l1 0 = nth n l2 0.
+Proof.
+  induction n.
+  - intros l1 l2 H. rewrite <- is_eq_veq in H.
+    destruct l1; destruct l2; simpl in *; reflect; auto; destruct H; auto.
+  - intros l1 l2 H. rewrite <- is_eq_veq in H.
+    destruct l1; destruct l2; simpl in *; reflect; auto; destruct H; auto.
+    + specialize (IHn nil l2). rewrite <- is_eq_veq in IHn. rewrite <- IHn by (destruct l2; auto). destruct n; auto.
+    + specialize (IHn l1 nil). rewrite <- is_eq_veq in IHn. rewrite IHn by (destruct l1; auto). destruct n; auto.
+Qed.
+
+Theorem generate_loop_preserves_sem :
+  forall d n pi st env mem1 mem2,
+    (d <= n)%nat ->
+    generate_loop d n pi = Ok st ->
+    loop_semantics st env mem1 mem2 ->
+    length env = (n - d)%nat ->
+    (forall c, In c pi.(pi_poly) -> fst c =v= resize n (fst c)) ->
+    (forall c, In c pi.(pi_poly) -> fst c =v= resize (n - d)%nat (fst c) -> satisfies_constraint (rev env) c = true) ->
+    env_poly_lex_semantics (rev env) n (pi :: nil) mem1 mem2.
+Proof.
+  induction d.
+  - intros n pi st env mem1 mem2 Hnd Hgen Hsem Hlen Hpilen Henvsat. simpl in *.
+    injection Hgen as Hgen.
+    unfold env_poly_lex_semantics.
+    eapply PolyLexProgress with (n := 0%nat) (p := rev env); [ |reflexivity| | | apply PolyLexDone].
+    + unfold env_scan. simpl. reflect. split; [split|].
+      * rewrite resize_eq; reflexivity.
+      * rewrite resize_eq; [reflexivity | rewrite rev_length; lia].
+      * unfold in_poly. rewrite forallb_forall. intros c Hin.
+        apply Henvsat; auto. rewrite Nat.sub_0_r. auto.
+    + intros n2 p2 Hcmp.
+      apply not_true_iff_false; intros H; apply env_scan_single in H; [|rewrite rev_length; lia].
+      rewrite H in Hcmp. rewrite lex_compare_reflexive in Hcmp. congruence.
+    + rewrite <- Hgen in Hsem. inversion_clear Hsem.
+      unfold affine_product in *. rewrite map_map in H.
+      erewrite map_ext in H; [exact H|].
+      intros; apply make_affine_expr_correct. lia.
+    + intros n1 p1. unfold scanned.
+      destruct n1 as [|n1]; [|destruct n1; simpl; auto]. simpl.
+      apply not_true_iff_false; intros H; reflect; destruct H as [H1 H2]; apply env_scan_single in H1; [|rewrite rev_length; lia].
+      rewrite H1 in H2; rewrite is_eq_reflexive in H2. destruct H2; congruence.
+  - intros n pi st env mem1 mem2 Hnd Hgen Hsem Hlen Hpilen Henvsat. simpl in *.
+    bind_ok_destruct Hgen proj Hproj. bind_ok_destruct Hgen lb Hlb. bind_ok_destruct Hgen ub Hub. bind_ok_destruct Hgen inner Hinner.
+    injection Hgen as Hgen. rewrite <- Hgen in Hsem.
+    inversion_clear Hsem.
+    unfold env_poly_lex_semantics in *.
+    eapply poly_lex_semantics_extensionality.
+    + apply poly_lex_concat_seq with (to_scans := fun x => env_scan (pi :: nil) (rev (x :: env)) n).
+      * eapply iter_semantics_map; [|apply H]. simpl.
+        intros x mem3 mem4 Hbounds Hloop. eapply IHd with (env := x :: env); simpl; eauto.
+        -- lia.
+        -- lia.
+        -- intros c Hin Heq.
+           destruct (project_reverse_inclusion (n - d)%nat (pi_poly pi) proj c Hproj Hin Heq) as [c' [Heqc' Hinc']].
+           replace (n - d)%nat with (S (n - S d))%nat in Heq by lia.
+           rewrite resize_succ in Heq.
+           destruct (nth (n - S d) (fst c) 0 =? 0) eqn:Hzero; reflect.
+           ++ rewrite Hzero in Heq.
+              setoid_replace (0 :: nil) with (@nil Z) in Heq by (rewrite <- is_eq_veq; auto).
+              unfold satisfies_constraint. rewrite Heq.
+              rewrite dot_product_app by (rewrite rev_length, resize_length; auto). simpl.
+              rewrite Z.add_0_r. rewrite app_nil_r in Heq. rewrite <- Heq.
+              apply Henvsat; auto.
+           ++ rewrite Heqc'. rewrite find_bounds_correct in Hbounds by eauto.
+              apply Hbounds; auto. erewrite nth_eq in Hzero; [exact Hzero|].
+              rewrite Heqc'; reflexivity.
+      * intros x. apply env_scan_proper.
+      * intros x1 x2 m p H1 H2. apply env_scan_begin in H1. apply env_scan_begin in H2.
+        assert (Heq : resize (length (rev (x1 :: env))) p = resize (length (rev (x2 :: env))) p).
+        { simpl. rewrite !app_length; simpl. auto. }
+        rewrite H1 in Heq at 1. rewrite H2 in Heq at 2.
+        rewrite !resize_app in Heq by auto.
+        assert (Heq2: rev (rev (x1 :: env)) = rev (rev (x2 :: env))) by (f_equal; auto).
+        rewrite !rev_involutive in Heq2; congruence.
+      * intros x1 n1 p1 x2 n2 p2 Hcmp H1 H2.
+        apply env_scan_begin in H1; apply env_scan_begin in H2.
+        rewrite H1 in Hcmp; rewrite H2 in Hcmp.
+        rewrite lex_compare_app in Hcmp by (rewrite !rev_length; simpl; auto).
+        simpl in Hcmp. rewrite lex_compare_app in Hcmp by auto.
+        rewrite lex_compare_reflexive in Hcmp. simpl in Hcmp.
+        destruct (x2 ?= x1) eqn:Hcmpx; reflect; [lia | lia | congruence].
+    + simpl. intros m p.
+      rewrite eq_iff_eq_true. rewrite existsb_exists.
+      rewrite env_scan_split by (rewrite rev_length; lia).
+      split.
+      * intros [x [H1 H2]]; exists x; assumption.
+      * intros [x Hscan]; exists x; split; [|auto].
+        rewrite Zrange_in. unfold env_scan in Hscan. destruct m; [|destruct m; simpl in Hscan; congruence].
+        simpl in Hscan. reflect.
+        destruct Hscan as [[Hscan1 Hscan2] Hscan3].
+        assert (Hinproj : in_poly (rev env ++ x :: nil) proj = true).
+        { rewrite Hscan1. eapply project_inclusion; [|apply Hscan3].
+          rewrite app_length; rewrite rev_length; rewrite Hlen; simpl.
+          rewrite <- Hproj. f_equal. lia.
+        }
+        rewrite find_bounds_correct by eauto.
+        unfold in_poly in Hinproj. rewrite forallb_forall in Hinproj.
+        intros; auto.
+Qed.
